@prefix dcterms: <http://purl.org/dc/terms/> .
@prefix ldp: <http://www.w3.org/ns/ldp#> .
@prefix ore: <http://www.openarchives.org/ore/terms/> .
@prefix owl: <http://www.w3.org/2002/07/owl#> .
@prefix pcdm: <http://pcdm.org/models#> .
@prefix rdf: <http://www.w3.org/1999/02/22-rdf-syntax-ns#> .
@prefix rdfs: <http://www.w3.org/2000/01/rdf-schema#> .
@prefix xsd: <http://www.w3.org/2001/XMLSchema#> .

pcdm:AdministrativeSet a rdfs:Class ;
    rdfs:label "Administrative Set"@en ;
    rdfs:comment """
        An Administrative Set is a grouping of resources that an administrative unit is ultimately
        responsible for managing. The set itself helps to manage the items within it. An Object
        or Collection may be contained by only one AdministrativeSet.
      """@en ;
    rdfs:isDefinedBy pcdm: ;
    rdfs:subClassOf ldp:Container .

pcdm:AlternateOrder a rdfs:Class ;
    rdfs:label "Alternate Order"@en ;
    rdfs:comment """
        An AlternateOrder is an alternate ordering of its parent's members.  It should only order the
        parent's members, and otherwise has all of the features of ordering (some members may be
        omitted from the order, members may appear more than once in the order, etc.).
      """@en ;
    rdfs:isDefinedBy pcdm: ;
    rdfs:subClassOf pcdm:Object .

pcdm:Collection a rdfs:Class ;
    rdfs:label "Collection"@en ;
    rdfs:comment """
        A Collection is a group of resources. Collections have descriptive metadata, access metadata,
        and may links to works and/or collections. By default, member works and collections are an
        unordered set, but can be ordered using the ORE Proxy class.
      """@en ;
    rdfs:isDefinedBy pcdm: ;
    rdfs:subClassOf ore:Aggregation .

pcdm:File a rdfs:Class ;
    rdfs:label "File"@en ;
    rdfs:comment """
        A File is a sequence of binary data and is described by some accompanying metadata.
        The metadata typically includes at least basic technical metadata (size, content type,
        modification date, etc.), but can also include properties related to preservation,
        digitization process, provenance, etc. Files MUST be contained by exactly one Object.
      """@en ;
    rdfs:isDefinedBy pcdm: .

pcdm:Object a rdfs:Class ;
    rdfs:label "Object"@en ;
    rdfs:comment """
        An Object is an intellectual entity, sometimes called a "work", "digital object", etc.
        Objects have descriptive metadata, access metadata, may contain files and other Objects as
        member "components". Each level of a work is therefore represented by an Object instance,
        and is capable of standing on its own, being linked to from Collections and other Objects.
        Member Objects can be ordered using the ORE Proxy class.
      """@en ;
    rdfs:isDefinedBy pcdm: ;
    rdfs:subClassOf ore:Aggregation .

pcdm:fileOf a rdf:Property ;
    rdfs:label "is file of"@en ;
    rdfs:comment "Links from a File to its containing Object."@en ;
    rdfs:domain pcdm:File ;
    rdfs:isDefinedBy pcdm: ;
    rdfs:range pcdm:Object ;
    rdfs:subPropertyOf ore:isAggregatedBy ;
    owl:inverseOf pcdm:hasFile .

pcdm:memberOf a rdf:Property ;
    rdfs:label "is member of"@en ;
    rdfs:comment "Links from an Object or Collection to a containing Object or Collection."@en ;
    rdfs:domain ore:Aggregation ;
    rdfs:isDefinedBy pcdm: ;
    rdfs:range ore:Aggregation ;
    rdfs:subPropertyOf ore:isAggregatedBy ;
    owl:inverseOf pcdm:hasMember .

pcdm:relatedObjectOf a rdf:Property ;
    rdfs:label "is related object of"@en ;
    rdfs:comment "Links from an Object to a Object or Collection that it is related to."@en ;
    rdfs:domain pcdm:Object ;
    rdfs:isDefinedBy pcdm: ;
    rdfs:range ore:Aggregation ;
    rdfs:subPropertyOf ore:isAggregatedBy ;
    owl:inverseOf pcdm:hasRelatedObject .

pcdm:hasFile a rdf:Property ;
    rdfs:label "has file"@en ;
    rdfs:comment "Links to a File contained by this Object."@en ;
    rdfs:domain pcdm:Object ;
    rdfs:isDefinedBy pcdm: ;
    rdfs:range pcdm:File ;
    rdfs:subPropertyOf ore:aggregates .

pcdm:hasMember a rdf:Property ;
    rdfs:label "has member"@en ;
    rdfs:comment """Links to a subsidiary Object or Collection. Typically used to link
          to component parts, such as a book linking to a page.  Note on transitivity: hasMember is
          not defined as transitive, but applications may treat it as transitive as local needs
          dictate."""@en ;
    rdfs:domain ore:Aggregation ;
    rdfs:isDefinedBy pcdm: ;
    rdfs:range ore:Aggregation ;
    rdfs:subPropertyOf ore:aggregates .

pcdm:hasRelatedObject a rdf:Property ;
    rdfs:label "has related object"@en ;
    rdfs:comment "Links to a related Object that is not a component part, such as an object representing a donor agreement or policies that govern the resource."@en ;
    rdfs:domain ore:Aggregation ;
    rdfs:isDefinedBy pcdm: ;
    rdfs:range pcdm:Object ;
    rdfs:subPropertyOf ore:aggregates .

pcdm: dcterms:modified "2015-10-14"^^xsd:date ;
    dcterms:publisher <http://www.duraspace.org/> ;
    dcterms:title "Portland Common Data Model"@en ;
    rdfs:comment "Ontology for the Portland Common Data Model, intended to underlie a wide array of repository and DAMS applications."@en ;
    rdfs:seeAlso <https://github.com/duraspace/pcdm/wiki> ;
    owl:priorVersion <http://pcdm.org/2015/09/28/models> ;
    owl:versionInfo "2015/10/14" .
